Bryan Heiser

2.a. This language contains a, b, and c in its alphabet. It must begin with a and end with a also.
There must be at least two a's in a string, but is not limited beyond that.
Additionally, b and c cannot be in the strings by themselves, they must be together in the string or not at all.
So, the strings must contain the same number of b's as c's. 

b. Sentences 1 and 4 are in the language generated by this grammar.
	1. baab
		S -> AaBb
  	     	  -> baBb
		  -> baab
	4. bbaab
		S -> AaBb
		  -> AbaBb
		  -> bbaBb
		  -> bbaab

c. Sentences 1 and 5 are in the language generated by this grammar.
	1. abcd
		S
	     | | | |
	     a S c B
	       |   |
	       b   d

	5. accc
		S
	     | | | |
	     a S c B
	       |   |
	       A   A
	       |   |
	       c   c

d. a ⊕ a ⊕ a  This is a sentence in the language generated by the given grammar.

There are two ways to generate this sentence with the grammar provided:
	A -> A ⊕ A			A -> A ⊕ A
	  -> a ⊕ A			  -> A ⊕ A ⊕ A
	  -> a ⊕ A ⊕ A		OR	  -> a ⊕ A ⊕ A
	  -> a ⊕ a ⊕ A			  -> a ⊕ a ⊕ A
	  -> a ⊕ a ⊕ a			  -> a ⊕ a ⊕ a

These two derivations show that there are two ways to construct the sentence a ⊕ a ⊕ a.
Given this sentence, it is unclear how the sentence was constructed; therefore, this grammar is ambiguous.

e. ???

3.a.
i. The expressions generated by both grammars will be like the binary expressions we are working with.
They will be expressions like 2 + 2 or nested expressions like 2 + (2 * 4).

ii. Both grammars generate expressions like operand operator operand all the way to operand operator operand operator operand operator operand ...
But the second grammar allows for just operand to be an expression generated.
So these two grammars produce different expressions.

b. To determine which operator ('-' or '<<') has a higher precedence I looked at the following expression: 7 - 3 << 2
Excecuting println(7 - 3 << 2) returns 16.
Looking at the output of println((7 - 3) << 2) and println(7 - (3 << 2)) they return 16 and -5, respectively.
So, it appears that '-' has a higher precedence than '<<'.

c. S ::= n.n|-n.n|n.m|-n.m|m.n|-m.n|m.m|e
e ::= n.nEn|-n.nEn|n.nE-n|-n.nE-n|m.nEn|-m.nEn|m.nE-n|-m.nE-n
n ::= 1|2|3|4|5|6|7|8|9|1n|2n|3n|4n|5n|6n|7n|8n|9n
m ::= 0|0m



